src/Noninterference/TransactionalDisk/HSS.v
@@ -134,6 +134,177 @@ cleanup; eauto;
 simpl; intuition eauto.
 Qed.
 
+Lemma have_same_structure_InodeAllocator_write:
+forall inum u u' s1 s2 v1 v2,
+(fun s1 s2  => exists s1a s2a, 
+File.files_inner_rep s1a (fst (snd (snd s1))) /\ 
+File.files_inner_rep s2a (fst (snd (snd s2))) /\ 
+FD_related_states u' None s1a s2a) s1 s2 ->
+have_same_structure
+(@lift_L2 AuthenticationOperation _ TD _ (Inode.InodeAllocator.write inum v1))
+(@lift_L2 AuthenticationOperation _ TD _ (Inode.InodeAllocator.write inum v2)) u s1 s2.
+Proof.
+unfold Inode.InodeAllocator.write; simpl; intros.
+destruct (Compare_dec.lt_dec inum Inode.InodeAllocatorParams.num_of_blocks); 
+simpl; intuition eauto.
+
+repeat invert_exec; try lia.
+unfold AD_related_states, refines_related in *; cleanup; simpl in *.
+unfold refines, File.files_rep, File.files_inner_rep  in *; cleanup.
+erewrite TSDelete.inode_allocations_are_same_2 in *; eauto.
+destruct_fresh (nth_error
+(value_to_bits
+   (fst (snd (snd s2)) Inode.InodeAllocatorParams.bitmap_addr)) inum);
+setoid_rewrite D.
+destruct b; simpl; intuition eauto.
+simpl; intuition eauto.
+destruct (block_allocator_empty inum); 
+cleanup; eauto;
+simpl; intuition eauto.
+Qed.
+
+
+Lemma have_same_structure_DiskAllocator_write:
+forall bn1 bn2 u u' s1 s2 v1 v2,
+(fun s1 s2  => exists s1a s2a, 
+File.files_inner_rep s1a (fst (snd (snd s1))) /\ 
+File.files_inner_rep s2a (fst (snd (snd s2))) /\ 
+FD_related_states u' None s1a s2a) s1 s2 ->
+(bn1 < File.DiskAllocatorParams.num_of_blocks <->
+bn2 < File.DiskAllocatorParams.num_of_blocks) ->
+(nth_error
+(value_to_bits
+   (fst (snd (snd s1))
+      File.DiskAllocatorParams.bitmap_addr)) bn1 = nth_error
+      (value_to_bits
+         (fst (snd (snd s2))
+            File.DiskAllocatorParams.bitmap_addr)) bn2) ->
+have_same_structure
+(@lift_L2 AuthenticationOperation _ TD _ (File.DiskAllocator.write bn1 v1))
+(@lift_L2 AuthenticationOperation _ TD _ (File.DiskAllocator.write bn2 v2)) u s1 s2.
+Proof.
+unfold File.DiskAllocator.write; simpl; intros.
+destruct (Compare_dec.lt_dec bn1 File.DiskAllocatorParams.num_of_blocks); 
+destruct (Compare_dec.lt_dec bn2 File.DiskAllocatorParams.num_of_blocks); 
+simpl; intuition eauto.
+
+repeat invert_exec; try lia.
+unfold AD_related_states, refines_related in *; cleanup; simpl in *.
+unfold refines, File.files_rep in *; cleanup.
+setoid_rewrite H1.
+destruct_fresh (nth_error (value_to_bits (fst (snd (snd s2)) File.DiskAllocatorParams.bitmap_addr)) bn2);
+setoid_rewrite D.
+destruct b; simpl; intuition eauto.
+simpl; intuition eauto.
+destruct (block_allocator_empty bn1); 
+destruct (block_allocator_empty bn2); 
+cleanup; eauto;
+simpl; intuition eauto.
+Qed.
+
+
+Lemma have_same_structure_DiskAllocator_alloc:
+forall u u' s1 s2 v1 v2,
+(fun s1 s2  => exists s1a s2a, 
+File.files_inner_rep s1a (fst (snd (snd s1))) /\ 
+File.files_inner_rep s2a (fst (snd (snd s2))) /\ 
+FD_related_states u' None s1a s2a) s1 s2 ->
+
+(get_first_zero_index
+   (firstn File.DiskAllocatorParams.num_of_blocks
+      (value_to_bits
+         (fst (snd (snd s1))
+            File.DiskAllocatorParams.bitmap_addr)))
+ < File.DiskAllocatorParams.num_of_blocks <-> 
+ get_first_zero_index
+ (firstn File.DiskAllocatorParams.num_of_blocks
+    (value_to_bits
+       (fst (snd (snd s2))
+          File.DiskAllocatorParams.bitmap_addr)))
+< File.DiskAllocatorParams.num_of_blocks) ->
+have_same_structure
+(@lift_L2 AuthenticationOperation _ TD _ (File.DiskAllocator.alloc v1))
+(@lift_L2 AuthenticationOperation _ TD _ (File.DiskAllocator.alloc v2)) u s1 s2.
+Proof.
+unfold File.DiskAllocator.alloc; simpl; intros.
+simpl; intuition eauto.
+
+repeat invert_exec; try lia.
+cleanup.
+unfold AD_related_states, refines_related in *; cleanup; simpl in *.
+unfold refines, File.files_rep in *; cleanup.
+destruct (Compare_dec.lt_dec
+(get_first_zero_index
+   (firstn
+      File.DiskAllocatorParams.num_of_blocks
+      (value_to_bits
+         (fst (snd (snd s1))
+            File.DiskAllocatorParams.bitmap_addr)))));
+destruct (Compare_dec.lt_dec
+(get_first_zero_index
+   (firstn
+      File.DiskAllocatorParams.num_of_blocks
+      (value_to_bits
+         (fst (snd (snd s2))
+            File.DiskAllocatorParams.bitmap_addr))))); try lia.
+
+
+simpl; intuition eauto.
+repeat invert_exec; try lia; cleanup.
+simpl; intuition eauto.
+destruct r1,r2; try solve [intuition congruence];
+simpl; eauto.
+destruct u0, u1; try solve [intuition congruence];
+simpl; eauto.
+destruct u0; try solve [intuition congruence];
+simpl; eauto.
+destruct u0; try solve [intuition congruence];
+simpl; eauto.
+{
+  pose proof File.DiskAllocatorParams.blocks_fit_in_disk.
+  pose proof File.DiskAllocatorParams.num_of_blocks_in_bounds.
+  unfold File.DiskAllocatorParams.bitmap_addr,
+  File.DiskAllocatorParams.num_of_blocks in *.
+  assert (S (get_first_zero_index
+  (firstn file_blocks_count (value_to_bits (fst (snd (snd s2)) file_blocks_start)))) <=
+file_blocks_count).
+lia.
+
+exfalso; eapply Lt.le_not_lt.
+2: apply H1.
+eapply PeanoNat.Nat.le_trans; eauto.
+eapply PeanoNat.Nat.add_le_mono; eauto.
+}
+try solve [intuition congruence];
+simpl; eauto.
+{
+  pose proof File.DiskAllocatorParams.blocks_fit_in_disk.
+  pose proof File.DiskAllocatorParams.num_of_blocks_in_bounds.
+  unfold File.DiskAllocatorParams.bitmap_addr,
+  File.DiskAllocatorParams.num_of_blocks in *.
+  assert (S (get_first_zero_index
+  (firstn file_blocks_count (value_to_bits (fst (snd (snd s1)) file_blocks_start)))) <=
+file_blocks_count).
+lia.
+
+exfalso; eapply Lt.le_not_lt.
+2: apply H1.
+eapply PeanoNat.Nat.le_trans; eauto.
+eapply PeanoNat.Nat.add_le_mono; eauto.
+}
+try solve [intuition congruence];
+simpl; eauto.
+try solve [intuition congruence];
+simpl; eauto.
+{
+  pose proof File.DiskAllocatorParams.blocks_fit_in_disk.
+  pose proof File.DiskAllocatorParams.num_of_blocks_in_bounds.
+  unfold File.DiskAllocatorParams.bitmap_addr,
+  File.DiskAllocatorParams.num_of_blocks in *; lia.
+}
+Qed.
+
+
 Lemma have_same_structure_get_inode:
 forall inum u u' s1 s2,
 (fun s1 s2  => exists s1a s2a, 
@@ -161,7 +332,20 @@ Unshelve.
 all: eauto.
 Qed.
 
-
+Lemma have_same_structure_set_inode:
+forall inum in1 in2 u u' s1 s2,
+(fun s1 s2  => exists s1a s2a, 
+File.files_inner_rep s1a (fst (snd (snd s1))) /\ 
+File.files_inner_rep s2a (fst (snd (snd s2))) /\ 
+FD_related_states u' None s1a s2a) s1 s2 ->
+have_same_structure
+(@lift_L2 AuthenticationOperation _ TD _ (Inode.set_inode inum in1))
+(@lift_L2 AuthenticationOperation _ TD _ (Inode.set_inode inum in2)) u s1 s2.
+Proof.
+unfold Inode.set_inode; simpl; intros.
+simpl; intuition eauto.
+eapply have_same_structure_InodeAllocator_write; eauto.
+Qed.
 
 Lemma have_same_structure_get_owner:
 forall inum u u' s1 s2,
@@ -210,6 +394,54 @@ unfold refines, File.files_rep in *; cleanup.
 eapply have_same_structure_get_inode; eauto.
 destruct r1,r2; try solve [intuition congruence];
 simpl; eauto.
+Unshelve.
+all: eauto.
+Qed.
+
+Lemma have_same_structure_Inode_extend:
+forall inum v1 v2 u u' s1 s2,
+(fun s1 s2  => exists s1a s2a, 
+File.files_inner_rep s1a (fst (snd (snd s1))) /\ 
+File.files_inner_rep s2a (fst (snd (snd s2))) /\ 
+FD_related_states u' None s1a s2a) s1 s2 ->
+have_same_structure
+(@lift_L2 AuthenticationOperation _ TD _ (Inode.extend inum v1))
+(@lift_L2 AuthenticationOperation _ TD _ (Inode.extend inum v2)) u s1 s2.
+Proof.
+Transparent Inode.extend.
+Opaque Inode.get_inode.
+unfold Inode.extend; simpl; intros.
+simpl; intuition eauto.
+
+unfold AD_related_states, refines_related in *; cleanup;
+simpl in *.
+unfold refines, File.files_rep in *; cleanup.
+eapply have_same_structure_get_inode; eauto.
+eapply lift2_invert_exec in H0.
+eapply lift2_invert_exec in H1; cleanup.
+apply HC_map_ext_eq in H1; subst.
+eapply_fresh Inode.get_inode_finished_oracle_eq in H5; eauto.
+destruct r1,r2; try solve [intuition congruence];
+simpl; eauto.
+eapply have_same_structure_set_inode.
+unfold File.files_inner_rep in *; cleanup.
+eapply Inode.get_inode_finished in H5; eauto.
+eapply Inode.get_inode_finished in H3; eauto.
+cleanup.
+clear H H5.
+
+unfold File.files_inner_rep; 
+do 2 eexists; intuition eauto.
+eexists; intuition eauto.
+eexists; intuition eauto.
+eapply File.DiskAllocator.block_allocator_rep_inbounds_eq; 
+eauto; intros; FileInnerSpecs.solve_bounds.
+
+unfold File.files_inner_rep; 
+do 2 eexists; intuition eauto.
+do 2 eexists; intuition eauto.
+eapply File.DiskAllocator.block_allocator_rep_inbounds_eq; 
+eauto; intros; FileInnerSpecs.solve_bounds.
 Unshelve.
 all: eauto.
 Qed.
@@ -340,6 +572,207 @@ simpl in *; try lia; try congruence.
 Qed.
 
 
+Lemma have_same_structure_write_inner:
+forall inum off u u' s1 s2 v1 v2,
+(fun s1 s2  => exists s1a s2a, 
+File.files_inner_rep s1a (fst (snd (snd s1))) /\ 
+File.files_inner_rep s2a (fst (snd (snd s2))) /\ 
+FD_related_states u' None s1a s2a) s1 s2 ->
+have_same_structure
+(@lift_L2 AuthenticationOperation _ TD _ (File.write_inner off v1 inum))
+(@lift_L2 AuthenticationOperation _ TD _ (File.write_inner off v2 inum)) u s1 s2.
+Proof.
+Transparent File.write_inner.
+Opaque Inode.get_block_number.
+unfold File.read_inner; simpl; intros.
+simpl; intuition eauto.
+
+eapply have_same_structure_get_block_number; eauto.
+eapply lift2_invert_exec in H0.
+eapply lift2_invert_exec in H1; cleanup.
+apply map_ext_eq in H1; subst.
+2: intros; cleanup; intuition congruence.
+unfold File.files_inner_rep in *; cleanup.
+eapply_fresh Inode.get_block_number_finished_oracle_eq in H5; eauto.
+cleanup; destruct r1,r2; try solve [intuition congruence];
+simpl; eauto.
+intuition.
+eapply Inode.get_block_number_finished in H5; eauto.
+eapply Inode.get_block_number_finished in H3; eauto.
+repeat split_ors; cleanup.
+
+eapply have_same_structure_DiskAllocator_write; eauto.
+clear H3 H5.
+do 2 eexists; intuition eauto.
+
+unfold File.files_inner_rep; 
+do 2 eexists; intuition eauto.
+do 2 eexists; intuition eauto.
+eapply File.DiskAllocator.block_allocator_rep_inbounds_eq; 
+eauto; intros; FileInnerSpecs.solve_bounds.
+
+unfold File.files_inner_rep; 
+do 2 eexists; intuition eauto.
+do 2 eexists; intuition eauto.
+eapply File.DiskAllocator.block_allocator_rep_inbounds_eq; 
+eauto; intros; FileInnerSpecs.solve_bounds.
+
+{
+  repeat split_ors; cleanup.
+  shelve.
+}
+{
+  repeat split_ors; cleanup.
+  shelve.
+}
+{
+  intros.
+  match goal with
+   | [H: _ ?inum = Some _,
+      H0: _ ?inum = Some _ |- _] =>
+   eapply_fresh FileInnerSpecs.inode_exists_then_file_exists in H; eauto; cleanup;
+   eapply_fresh FileInnerSpecs.inode_exists_then_file_exists in H0; eauto; cleanup
+   end.
+   unfold FD_related_states,
+   same_for_user_except in *; cleanup.
+   match goal with
+   | [H: ?fm1 ?inum = Some _,
+      H0: ?fm2 ?inum = Some _,
+      H1: forall (_: addr) (_ _: File), 
+       ?fm1 _ = Some _ ->
+       ?fm2 _ = Some _ ->
+       _ = _ /\ _ = _ |- _] =>
+       eapply_fresh H1 in H; eauto; cleanup
+  end.
+   unfold File.file_map_rep in *; cleanup.
+   match goal with
+   | [H: ?x1 ?inum = Some _,
+      H0: ?x2 ?inum = Some _,
+      H1: forall (_: Inode.Inum) _ _, 
+      ?x1 _ = Some _ ->
+      _ _ = Some _ -> _,
+      H2: forall (_: Inode.Inum) _ _, 
+      ?x2 _ = Some _ ->
+      _ _ = Some _ -> _ |- _] =>
+      eapply H1 in H; eauto; cleanup;
+      eapply H2 in H0; eauto; cleanup
+   end.
+   unfold File.file_rep in *; cleanup; eauto.
+}
+
+Unshelve.
+all: eauto.
+{
+  intuition eauto.
+  eapply SameRetType.all_block_numbers_in_bound in H21.
+  3: eauto.
+  all: eauto.
+  eapply Forall_forall in H21; eauto.
+  apply in_seln; eauto.
+
+  eapply SameRetType.all_block_numbers_in_bound in H23.
+  2: eauto.
+  all: eauto.
+  eapply Forall_forall in H23; eauto.
+  apply in_seln; eauto.
+
+  eapply File.DiskAllocator.block_allocator_rep_inbounds_eq; eauto.
+  intros; FileInnerSpecs.solve_bounds.
+}
+{
+destruct (Compare_dec.lt_dec inum Inode.InodeAllocatorParams.num_of_blocks).
+- repeat erewrite TSCommon.used_blocks_are_allocated_2; eauto.
+all: eapply File.DiskAllocator.block_allocator_rep_inbounds_eq; eauto;
+intros; FileInnerSpecs.solve_bounds.
+- unfold Inode.inode_rep, Inode.inode_map_rep,
+Inode.inode_map_valid,
+Inode.inode_valid,
+Inode.InodeAllocator.block_allocator_rep in *; cleanup.
+
+rewrite H34, H39 in *; 
+simpl in *; try lia; try congruence.
+}
+Qed.
+
+
+Lemma have_same_structure_extend_inner:
+forall inum u u' s1 s2 v1 v2,
+(fun s1 s2  => exists s1a s2a, 
+File.files_inner_rep s1a (fst (snd (snd s1))) /\ 
+File.files_inner_rep s2a (fst (snd (snd s2))) /\ 
+FD_related_states u' None s1a s2a) s1 s2 ->
+have_same_structure
+(@lift_L2 AuthenticationOperation _ TD _ (File.extend_inner v1 inum))
+(@lift_L2 AuthenticationOperation _ TD _ (File.extend_inner v2 inum)) u s1 s2.
+Proof.
+Transparent File.extend_inner.
+Opaque Inode.get_block_number Inode.extend File.DiskAllocator.alloc.
+unfold File.extend_inner. simpl; intros.
+simpl; intuition eauto.
+
+eapply have_same_structure_DiskAllocator_alloc; eauto.
+cleanup; eapply InodeTS.free_block_exists_iff; eauto.
+eapply lift2_invert_exec in H0.
+eapply lift2_invert_exec in H1; cleanup.
+apply HC_map_ext_eq in H1; subst.
+unfold File.files_inner_rep, Inode.inode_rep in *; cleanup.
+eapply_fresh File.DiskAllocator.alloc_finished_oracle_eq in H5; eauto.
+cleanup; destruct r1,r2; try solve [intuition congruence];
+simpl; eauto.
+eapply have_same_structure_Inode_extend; eauto.
+
+eapply File.DiskAllocator.alloc_finished in H3; eauto.
+eapply File.DiskAllocator.alloc_finished in H5; eauto.
+repeat (repeat split_ors; cleanup).
+repeat cleanup_pairs.
+
+unfold File.files_inner_rep, Inode.inode_rep in *; cleanup;
+do 2 eexists; intuition eauto.
+eexists; intuition eauto.
+eexists; split.
+eapply Inode.InodeAllocator.block_allocator_rep_inbounds_eq.
+apply H.
+eauto; intros; FileInnerSpecs.solve_bounds.
+eauto.
+eexists; intuition eauto.
+{
+  unfold File.file_map_rep in *; cleanup; intuition eauto.
+  eapply_fresh H10 in H13; eauto.
+  unfold File.file_rep in *; cleanup.
+  intuition eauto.
+  erewrite Mem.upd_ne; eauto.
+
+  intuition; cleanup.
+  unfold Inode.inode_map_rep,
+  Inode.inode_map_valid,
+  Inode.inode_valid in *; cleanup.
+  eapply H26 in H27; cleanup.
+}
+
+unfold File.files_inner_rep; 
+do 2 eexists; intuition eauto.
+do 2 eexists; intuition eauto.
+eapply Inode.InodeAllocator.block_allocator_rep_inbounds_eq; 
+eauto; intros; FileInnerSpecs.solve_bounds.
+eexists; intuition eauto.
+{
+  unfold File.file_map_rep in *; cleanup; intuition eauto.
+  eapply_fresh H5 in H13; eauto.
+  unfold File.file_rep in *; cleanup.
+  intuition eauto.
+  erewrite Mem.upd_ne; eauto.
+
+  intuition; cleanup.
+  unfold Inode.inode_map_rep,
+  Inode.inode_map_valid,
+  Inode.inode_valid in *; cleanup.
+  eapply H26 in H27; cleanup.
+}
+
+Unshelve.
+all: eauto.
+Qed.
+
 Lemma get_owner_related_ret_eq:
 forall u u' ex s1 s2 o s1' s2' r1 r2 inum, 
 AD_related_states u' ex s1 s2 ->
@@ -385,36 +818,64 @@ Proof.
 Qed.
 
 
-Lemma have_same_structure_read:
-forall inum off u u' s1 s2,
+Lemma have_same_structure_auth_then_exec:
+forall T (p1 p2: _ -> TD.(prog) (option T)) inum u u' s1 s2,
+(forall s1 s2, 
+(fun s1 s2  => exists s1a s2a, 
+File.files_inner_rep s1a (fst (snd (snd s1))) /\ 
+File.files_inner_rep s2a (fst (snd (snd s2))) /\ 
+FD_related_states u' None s1a s2a) s1 s2 ->
+
+have_same_structure
+(@lift_L2 AuthenticationOperation _ TD _ (p1 inum))
+(@lift_L2 AuthenticationOperation _ TD _ (p2 inum)) u s1 s2) ->
+
+(forall (fm1 fm2 : disk File)
+(o : oracle' (TransactionalDiskLayer.TDCore data_length))
+(o' o1
+ o2 : list
+        (Language.token' (TransactionalDiskLayer.TDCore data_length)))
+(s1 : Language.state' (TransactionalDiskLayer.TDCore data_length))
+(s2 : txn_state * (total_mem * total_mem))
+(s1'
+ s2' : Language.state' (TransactionalDiskLayer.TDCore data_length))
+(r1 r2 : option T) (inum : nat),
+exec TD u o s1 (p1 inum) (Finished s1' r1) ->
+o ++ o1 = o' ++ o2 ->
+File.files_inner_rep fm1 (fst (snd s1)) ->
+File.files_inner_rep fm2 (fst (snd s2)) ->
+same_for_user_except u' None fm1 fm2 ->
+exec TD u o' s2 (p2 inum) (Finished s2' r2) ->
+o = o' /\ (r1 = None <-> r2 = None)) ->
+
 AD_related_states u' None s1 s2 ->
-have_same_structure (File.read inum off) (File.read inum off) u s1 s2.
+have_same_structure (File.auth_then_exec inum p1) (File.auth_then_exec inum p2) u s1 s2.
 Proof.
-  Opaque File.read_inner Inode.get_owner.
-  unfold File.read, File.auth_then_exec.
+  Opaque Inode.get_owner.
+  unfold File.auth_then_exec.
   intros; simpl.
   intuition eauto.
   eapply have_same_structure_get_owner; eauto.
 
-  eapply lift2_invert_exec in H0.
-eapply lift2_invert_exec in H1; cleanup.
-apply HC_map_ext_eq in H1; subst.
-eapply_fresh get_owner_related_ret_eq in H3; eauto.
+  eapply lift2_invert_exec in H2.
+eapply lift2_invert_exec in H3; cleanup.
+apply HC_map_ext_eq in H3; subst.
+eapply_fresh get_owner_related_ret_eq in H5; eauto.
 
 unfold AD_related_states, refines_related in *; 
 simpl in *; cleanup.
 
 unfold refines, File.files_rep in *; cleanup.
-rewrite <- H6, <- H8 in *; clear H6 H8.
+rewrite <- H8, <- H10 in *; clear H8 H10.
 unfold File.files_inner_rep in *; cleanup.
+eapply Inode.get_owner_finished in H7; eauto.
 eapply Inode.get_owner_finished in H5; eauto.
-eapply Inode.get_owner_finished in H3; eauto.
 repeat split_ors; cleanup.
 
-clear H3 H5. destruct r2; simpl; intuition eauto.
+clear H5 H7. destruct r2; simpl; intuition eauto.
 repeat invert_exec; intuition.
 simpl; intuition eauto.
-eapply have_same_structure_read_inner; eauto.
+apply H; eauto.
 do 2 eexists; intuition eauto.
 
 unfold File.files_inner_rep; eexists; intuition eauto.
@@ -427,12 +888,13 @@ eexists; intuition eauto.
 eapply File.DiskAllocator.block_allocator_rep_inbounds_eq; eauto.
 intros; SameRetType.solve_bounds.
 
-eapply lift2_invert_exec in H3.
-eapply lift2_invert_exec in H5; cleanup.
-apply HC_map_ext_eq in H5; subst.
+eapply lift2_invert_exec in H5.
+eapply lift2_invert_exec in H7; cleanup.
+apply HC_map_ext_eq in H7; subst.
 unfold FD_related_states  in *.
-eapply SameRetType.read_inner_finished_oracle_eq in H21. 
-2: eapply H24. 
+
+eapply H0 in H23. 
+2: eapply H26. 
 all: eauto.
 cleanup. 
 destruct r1, r2; simpl; intuition congruence.
@@ -450,4 +912,39 @@ intros; SameRetType.solve_bounds.
 simpl; intuition eauto.
 Unshelve.
 eauto.
+Qed.
+
+
+(** HSS for syscalls **)
+Lemma have_same_structure_read:
+forall inum off u u' s1 s2,
+AD_related_states u' None s1 s2 ->
+have_same_structure (File.read inum off) (File.read inum off) u s1 s2.
+Proof.
+  unfold File.read; intros.
+  eapply have_same_structure_auth_then_exec; eauto.
+  intros; eapply have_same_structure_read_inner; eauto.
+ intros; eapply SameRetType.read_inner_finished_oracle_eq; eauto. 
+Qed.
+
+Lemma have_same_structure_write:
+forall inum off u u' s1 s2 v1 v2,
+AD_related_states u' None s1 s2 ->
+have_same_structure (File.write inum off v1) (File.write inum off v2) u s1 s2.
+Proof.
+  unfold File.write; intros.
+  eapply have_same_structure_auth_then_exec; eauto.
+  intros; eapply have_same_structure_write_inner; eauto.
+ intros; eapply SameRetType.write_inner_finished_oracle_eq; eauto. 
+Qed.
+
+Lemma have_same_structure_extend:
+forall inum u u' s1 s2 v1 v2,
+AD_related_states u' None s1 s2 ->
+have_same_structure (File.extend inum v1) (File.extend inum v2) u s1 s2.
+Proof.
+  unfold File.extend; intros.
+  eapply have_same_structure_auth_then_exec; eauto.
+  intros; eapply have_same_structure_extend_inner; eauto.
+ intros; eapply SameRetType.extend_inner_finished_oracle_eq; eauto. 
 Qed.
