src/Noninterference/TransactionalDisk/Not_Init.v
@@ -4,6 +4,22 @@ Require Import ATCLayer ATC_Simulation ATC_AOE.
 
 Import FileDiskLayer.
 
+Ltac not_init_solve:= 
+  match goal with
+  | [H: eq_dep _ _ _ _ _ _ |- _] =>
+  inversion H
+  | [|- context [match ?x with | _ => _ end] ] =>
+  destruct x; simpl; intuition eauto
+  | [|- not_init _] =>
+  unfold 
+  Inode.set_inode,
+  File.DiskAllocator.read, 
+  Inode.InodeAllocator.read,
+  File.DiskAllocator.write,
+  Inode.InodeAllocator.write; simpl; intuition eauto
+  end.
+
+(*  
 Lemma not_init_InodeAllocator_read:
 forall inum,
 not_init (@lift_L2 AuthenticationOperation _ TD _(Inode.InodeAllocator.read inum)).
@@ -23,6 +39,20 @@ forall bn,
 not_init (@lift_L2 AuthenticationOperation _ TD _(File.DiskAllocator.read bn)).
 Proof.
   unfold File.DiskAllocator.read; simpl; intros.
+  destruct (Compare_dec.lt_dec bn File.DiskAllocatorParams.num_of_blocks).
+  simpl; intuition eauto.
+  inversion H.
+  destruct (nth_error (value_to_bits t) bn); simpl; intuition eauto.
+  destruct b; simpl; intuition eauto.
+  inversion H.
+  simpl; eauto.
+Qed.
+
+Lemma not_init_DiskAllocator_write:
+forall bn v,
+not_init (@lift_L2 AuthenticationOperation _ TD _(File.DiskAllocator.write bn v)).
+Proof.
+  unfold File.DiskAllocator.write; simpl; intros.
   destruct (Compare_dec.lt_dec bn File.DiskAllocatorParams.num_of_blocks).
   simpl; intuition eauto.
   inversion H.
@@ -76,19 +106,27 @@ Proof.
   apply not_init_DiskAllocator_read.
   destruct t; simpl; intuition eauto.
 Qed.
+*)
 
-
+Transparent Inode.get_owner Inode.get_block_number Inode.extend Inode.set_inode.
 Lemma not_init_read:
 forall inum off,
 not_init (FD.refinement.(Simulation.Definitions.compile) (FDOp.(Op) (Read inum off))).
 Proof.
-  Opaque Inode.get_owner File.read_inner.
-  simpl; intros; intuition eauto.
-  apply not_init_get_owner.
-  destruct t; simpl; intuition eauto.
-  destruct t; simpl; intuition eauto.
-  destruct u0; simpl; intuition eauto.
-  apply not_init_read_inner.
-  destruct t; simpl; intuition eauto.
-  all: inversion H.
+  intros; repeat not_init_solve.
+Qed.
+
+
+Lemma not_init_write:
+forall inum off v,
+not_init (FD.refinement.(Simulation.Definitions.compile) (FDOp.(Op) (Write inum off v))).
+Proof.
+  intros; repeat not_init_solve.
+Qed.
+
+Lemma not_init_extend:
+forall inum v,
+not_init (FD.refinement.(Simulation.Definitions.compile) (FDOp.(Op) (Extend inum v))).
+Proof.
+  intros; repeat not_init_solve.
 Qed.
